Update program simulation relation w.r.t. new specification.

common/ProgramSim.v
@@ -4,6 +4,7 @@ Require Import Coqlib Coqlib_linker.
 Require Import Maps_linker.
 Require Import Integers Floats Values AST Globalenvs.
 Require Import LinkerSpecification.
+Require Import Errors.
 
 Set Implicit Arguments.
 
@@ -11,15 +12,17 @@ Set Implicit Arguments.
 (* properties of linker *)
 Section LINKER_PROP.
 
-Variable (F V:Type).  
+Variable (Fundef F EF V:Type).
+Variable (fundef_dec: FundefDec Fundef F EF).
+Variable (EF_dec: forall (v1 v2:EF), {v1 = v2} + {v1 <> v2}).
 Variable (V_dec: forall (v1 v2:V), {v1 = v2} + {v1 <> v2}).
 
-Lemma gflink_globdefs defs1 defs2 (Hlink: @link_globdefs F V V_dec defs1 defs2 = None):
+Lemma gflink_globdefs defs1 defs2 (Hlink: link_globdefs fundef_dec EF_dec V_dec defs1 defs2 = None):
   exists var def1 def2,
     PTree.get var defs1 = Some def1 /\
     PTree.get var defs2 = Some def2 /\
-    ~ globdef_linkable def1 def2 /\
-    ~ globdef_linkable def2 def1.
+    ~ globdef_linkable fundef_dec def1 def2 /\
+    ~ globdef_linkable fundef_dec def2 def1.
 Proof.
   unfold link_globdefs in Hlink.
   match goal with
@@ -30,17 +33,17 @@ Proof.
   destruct Hlinkable as [i [x [Hx1 Hx2]]].
   destruct x; inv Hx2. rewrite PTree.gcombine in Hx1; auto.
   destruct (defs1 ! i) eqn:Hi1, (defs2 ! i) eqn:Hi2; inv Hx1.
-  destruct (globdef_linkable_dec V_dec g g0); inv H0.
-  destruct (globdef_linkable_dec V_dec g0 g); inv H1.
+  destruct (globdef_linkable_dec fundef_dec EF_dec V_dec g g0); inv H0.
+  destruct (globdef_linkable_dec fundef_dec EF_dec V_dec g0 g); inv H1.
   repeat eexists; eauto.
 Qed.
 
-Lemma gtlink_globdefs defs1 defs2 defs (Hlink: @link_globdefs F V V_dec defs1 defs2 = Some defs):
+Lemma gtlink_globdefs defs1 defs2 defs (Hlink: link_globdefs fundef_dec EF_dec V_dec defs1 defs2 = Some defs):
   forall var,
     match PTree.get var defs1, PTree.get var defs2, PTree.get var defs with
       | Some g1, Some g2, Some g =>
-        (globdef_linkable g1 g2 /\ g2 = g) \/
-        (globdef_linkable g2 g1 /\ g1 = g)
+        (globdef_linkable fundef_dec g1 g2 /\ g2 = g) \/
+        (globdef_linkable fundef_dec g2 g1 /\ g1 = g)
       | Some g1, None, Some g => g1 = g
       | None, Some g2, Some g => g2 = g
       | None, None, None => True
@@ -54,16 +57,16 @@ Proof.
   end.
   rewrite PTree.goption_map, PTree.gcombine; auto.
   destruct (defs1 ! i) eqn:Hi1, (defs2 ! i) eqn:Hi2; auto.
-  destruct (globdef_linkable_dec V_dec g g0).
+  destruct (globdef_linkable_dec fundef_dec EF_dec V_dec g g0).
   { left. split; auto. }
-  destruct (globdef_linkable_dec V_dec g0 g).
+  destruct (globdef_linkable_dec fundef_dec EF_dec V_dec g0 g).
   { right. split; auto. }
   eapply PTree_Properties.for_all_correct in Hlinkable; eauto.
   { instantiate (1 := None) in Hlinkable. inv Hlinkable. }
   instantiate (1 := i). rewrite PTree.gcombine; auto.
   rewrite Hi1, Hi2.
-  destruct (globdef_linkable_dec V_dec g g0); try (contradict n; auto; fail).
-  destruct (globdef_linkable_dec V_dec g0 g); try (contradict n0; auto; fail).
+  destruct (globdef_linkable_dec fundef_dec EF_dec V_dec g g0); try (contradict n; auto; fail).
+  destruct (globdef_linkable_dec fundef_dec EF_dec V_dec g0 g); try (contradict n0; auto; fail).
   auto.
 Qed.
 
@@ -73,31 +76,46 @@ End LINKER_PROP.
 (* lifting function simulation to program simulation *)
 Section PROGRAM_SIM.
 
-Variable (F_src F_tgt V:Type).
-Variable (V_dec: forall (v1 v2:V), {v1 = v2} + {v1 <> v2}).
+Variable (Fundef_src F_src EF_src V_src:Type).
+Variable (fundef_src_dec: FundefDec Fundef_src F_src EF_src).
+Variable (EF_src_dec: forall (v1 v2:EF_src), {v1 = v2} + {v1 <> v2}).
+Variable (V_src_dec: forall (v1 v2:V_src), {v1 = v2} + {v1 <> v2}).
+
+Variable (Fundef_tgt F_tgt EF_tgt V_tgt:Type).
+Variable (fundef_tgt_dec: FundefDec Fundef_tgt F_tgt EF_tgt).
+Variable (EF_tgt_dec: forall (v1 v2:EF_tgt), {v1 = v2} + {v1 <> v2}).
+Variable (V_tgt_dec: forall (v1 v2:V_tgt), {v1 = v2} + {v1 <> v2}).
+
+Variable (transf_EF: forall (ef:EF_src), res EF_tgt).
+Variable (transf_V: forall (v:V_src), res V_tgt).
+Definition V_sim (v_src:V_src) (v_tgt:V_tgt) := transf_V v_src = OK v_tgt.
 
 Parameter F_sim: forall (f_src:F_src) (f_tgt:F_tgt), Prop.
 
-Inductive globfun_sim: forall (g_src:AST.fundef F_src) (g_tgt:AST.fundef F_tgt), Prop :=
+Inductive globfun_sim (g_src:Fundef_src) (g_tgt:Fundef_tgt): Prop :=
 | globfun_sim_i
     f_src f_tgt
-    (Hf: F_sim f_src f_tgt):
-    globfun_sim (Internal f_src) (Internal f_tgt)
-| globfun_sim_e e:
-    globfun_sim (External e) (External e)
+    (Hsrc: fundef_src_dec g_src = inl f_src)
+    (Htgt: fundef_tgt_dec g_tgt = inl f_tgt)
+    (Hsim: F_sim f_src f_tgt)
+| globfun_sim_e
+    ef_src ef_tgt (Hef: transf_EF ef_src = OK ef_tgt)
+    (Hsrc: fundef_src_dec g_src = inr ef_src)
+    (Htgt: fundef_tgt_dec g_tgt = inr ef_tgt)
 .
 
-Inductive globdef_sim: forall (g_src:globdef (AST.fundef F_src) V) (g_tgt:globdef (AST.fundef F_tgt) V), Prop :=
+Inductive globdef_sim: forall (g_src:globdef Fundef_src V_src) (g_tgt:globdef Fundef_tgt V_tgt), Prop :=
 | globdef_sim_fun
     f_src f_tgt (Hf: globfun_sim f_src f_tgt):
     globdef_sim (Gfun f_src) (Gfun f_tgt)
-| globdef_sim_var v:
-    globdef_sim (Gvar v) (Gvar v)
+| globdef_sim_var
+    v_src v_tgt (Hv: transf_globvar transf_V v_src = OK v_tgt):
+    globdef_sim (Gvar v_src) (Gvar v_tgt)
 .
 
 Definition globdefs_sim
-           (defs_src:PTree.t (globdef (AST.fundef F_src) V))
-           (defs_tgt:PTree.t (globdef (AST.fundef F_tgt) V)):
+           (defs_src:PTree.t (globdef Fundef_src V_src))
+           (defs_tgt:PTree.t (globdef Fundef_tgt V_tgt)):
   Prop :=
   forall i,
     match PTree.get i defs_src, PTree.get i defs_tgt with
@@ -107,8 +125,8 @@ Definition globdefs_sim
     end.
 
 Definition globdef_list_sim
-           (defs_src:list (positive * globdef (AST.fundef F_src) V))
-           (defs_tgt:list (positive * globdef (AST.fundef F_tgt) V)):
+           (defs_src:list (positive * globdef Fundef_src V_src))
+           (defs_tgt:list (positive * globdef Fundef_tgt V_tgt)):
   Prop :=
   list_forall2
     (fun g_src g_tgt =>
@@ -117,13 +135,13 @@ Definition globdef_list_sim
     defs_src defs_tgt.
 
 Definition program_sim
-           (p_src:program (AST.fundef F_src) V) (p_tgt:program (AST.fundef F_tgt) V): Prop :=
+           (p_src:program Fundef_src V_src) (p_tgt:program Fundef_tgt V_tgt): Prop :=
   globdef_list_sim p_src.(prog_defs) p_tgt.(prog_defs) /\
   p_src.(prog_main) = p_tgt.(prog_main).
 
 Lemma globdefs_sim_globdef_list_sim
-      (defs_src: PTree.t (globdef (AST.fundef F_src) V))
-      (defs_tgt: PTree.t (globdef (AST.fundef F_tgt) V))
+      (defs_src: PTree.t (globdef Fundef_src V_src))
+      (defs_tgt: PTree.t (globdef Fundef_tgt V_tgt))
       (Hsim: globdefs_sim defs_src defs_tgt):
   globdef_list_sim (PTree.elements defs_src) (PTree.elements defs_tgt).
 Proof.
@@ -137,8 +155,8 @@ Proof.
 Qed.
 
 Lemma globdef_list_sim_globdefs_sim
-      (defs_src: list (positive * globdef (AST.fundef F_src) V))
-      (defs_tgt: list (positive * globdef (AST.fundef F_tgt) V))
+      (defs_src: list (positive * globdef Fundef_src V_src))
+      (defs_tgt: list (positive * globdef Fundef_tgt V_tgt))
       (Hsim: globdef_list_sim defs_src defs_tgt):
   globdefs_sim (PTree.unelements defs_src) (PTree.unelements defs_tgt).
 Proof.
@@ -152,17 +170,31 @@ Proof.
   apply IHl. auto.
 Qed.
 
+Ltac simplify_decs :=
+  repeat
+    match goal with
+      | [Hl: fundef_src_dec ?f = _,
+         Hr: fundef_src_dec ?f = _ |- _] =>
+        rewrite Hl in Hr; inv Hr
+      | [Hl: fundef_tgt_dec ?f = _,
+         Hr: fundef_tgt_dec ?f = _ |- _] =>
+        rewrite Hl in Hr; inv Hr
+      | [Hl: transf_EF ?ef = _,
+         Hr: transf_EF ?ef = _ |- _] =>
+        rewrite Hl in Hr; inv Hr
+    end.
+
 Lemma link_globdefs_sim
-      (defs1_src defs2_src:PTree.t (globdef (AST.fundef F_src) V))
-      (defs1_tgt defs2_tgt:PTree.t (globdef (AST.fundef F_tgt) V))
-      defs_src (Hdefs_src: link_globdefs V_dec defs1_src defs2_src = Some defs_src)
+      (defs1_src defs2_src:PTree.t (globdef Fundef_src V_src))
+      (defs1_tgt defs2_tgt:PTree.t (globdef Fundef_tgt V_tgt))
+      defs_src (Hdefs_src: link_globdefs fundef_src_dec EF_src_dec V_src_dec defs1_src defs2_src = Some defs_src)
       (H1: globdefs_sim defs1_src defs1_tgt)
       (H2: globdefs_sim defs2_src defs2_tgt):
   exists defs_tgt,
-    link_globdefs V_dec defs1_tgt defs2_tgt = Some defs_tgt /\
+    link_globdefs fundef_tgt_dec EF_tgt_dec V_tgt_dec defs1_tgt defs2_tgt = Some defs_tgt /\
     globdefs_sim defs_src defs_tgt.
 Proof.
-  destruct (link_globdefs V_dec defs1_tgt defs2_tgt) eqn:Hdefs_tgt.
+  destruct (link_globdefs fundef_tgt_dec EF_tgt_dec V_tgt_dec defs1_tgt defs2_tgt) eqn:Hdefs_tgt.
   { eexists. split; [eauto|].
     intro i. rename t into defs_tgt.
     eapply gtlink_globdefs in Hdefs_src. instantiate (1 := i) in Hdefs_src.
@@ -172,18 +204,20 @@ Proof.
     destruct (defs1_tgt ! i) eqn:Hi1_tgt, (defs2_tgt ! i) eqn:Hi2_tgt, (defs_tgt ! i) eqn:Hi_tgt; subst; try (inv Hdefs_tgt; fail);
     try (inv H1; fail); try (inv H2; fail); auto.
     destruct Hdefs_src as [[]|[]], Hdefs_tgt as [[]|[]]; subst; auto.
-    { inv H; inv H1; inv H2; inv H3; inv Hv; inv Hv0; try inv Hf; try inv Hf0.
-      { repeat constructor. }
-      { destruct v1, v2; simpl in *.
-        rewrite Hinfo, Hinit, Hinit0, Hreadonly, Hvolatile.
-        constructor.
+    { inv H; inv H1; inv H2; inv H3; inv Hv; inv Hv0; try inv Hf; try inv Hf0; simplify_decs.
+      { repeat constructor. eapply globfun_sim_e; eauto. }
+      { constructor. destruct v1, v2. simpl in *. subst.
+        unfold transf_globvar in *. simpl in *.
+        destruct (transf_V gvar_info0); inv H0. simpl in *.
+        inv Hv1. inv Hv2. simpl in *. subst. auto.
       }
     }
-    { inv H; inv H1; inv H2; inv H3; inv Hv; inv Hv0; try inv Hf; try inv Hf0.
-      { repeat constructor. }
-      { destruct v1, v2; simpl in *.
-        rewrite Hinfo, Hinit, Hinit0, Hreadonly, Hvolatile.
-        constructor.
+    { inv H; inv H1; inv H2; inv H3; inv Hv; inv Hv0; try inv Hf; try inv Hf0; simplify_decs.
+      { repeat constructor. eapply globfun_sim_e; eauto. }
+      { constructor. destruct v1, v2. simpl in *. subst.
+        unfold transf_globvar in *. simpl in *.
+        destruct (transf_V gvar_info0); inv H0. simpl in *.
+        inv Hv1. inv Hv2. simpl in *. subst. auto.
       }
     }
   }
@@ -198,39 +232,45 @@ Proof.
     rewrite Hi1_src, Hi2_src in Hdefs_src.
     destruct (defs_src ! i) eqn:Hi_src; [|inv Hdefs_src].
     destruct Hdefs_src as [[]|[]]; subst.
-    { inv H1; inv H2; inv H; try inv Hf; try inv Hf0.
-      { inv Hv. }
-      { inv Hv. }
-      { contradict H12. repeat constructor. }
-      { inv Hv. contradict H12. repeat constructor. }
-      { contradict H12. constructor. auto. }
+    { inv H1; inv H2; inv H; inv Hv; try inv Hv0; try inv Hf; try inv Hf0; simplify_decs.
+      { contradict H12. constructor. eapply globfun_linkable_ei; eauto. }
+      { contradict H12. constructor. eapply globfun_linkable_ee; eauto. }
+      { contradict H12. constructor.
+        destruct v_src, v_src0. inv Hv1. simpl in *. subst.
+        unfold transf_globvar in *. simpl in *.
+        destruct (transf_V gvar_info0); inv H0; inv H1.
+        constructor; auto.
+      }
     }
-    { inv H1; inv H2; inv H; try inv Hf; try inv Hf0.
-      { inv Hv. }
-      { contradict H21. repeat constructor. }
-      { inv Hv. }
-      { inv Hv. contradict H12. repeat constructor. }
-      { contradict H21. constructor. auto. }
+    { inv H1; inv H2; inv H; inv Hv; try inv Hv0; try inv Hf; try inv Hf0; simplify_decs.
+      { contradict H21. constructor. eapply globfun_linkable_ei; eauto. }
+      { contradict H21. constructor. eapply globfun_linkable_ee; eauto. }
+      { contradict H21. constructor.
+        destruct v_src, v_src0. inv Hv1. simpl in *. subst.
+        unfold transf_globvar in *. simpl in *.
+        destruct (transf_V gvar_info); inv H0; inv H1.
+        constructor; auto.
+      }
     }
   }
 Qed.
 
 Lemma link_globdef_list_sim
-      (defs1_src defs2_src:list (positive * globdef (AST.fundef F_src) V))
-      (defs1_tgt defs2_tgt:list (positive * globdef (AST.fundef F_tgt) V))
-      defs_src (Hdefs_src: link_globdef_list V_dec defs1_src defs2_src = Some defs_src)
+      (defs1_src defs2_src:list (positive * globdef Fundef_src V_src))
+      (defs1_tgt defs2_tgt:list (positive * globdef Fundef_tgt V_tgt))
+      defs_src (Hdefs_src: link_globdef_list fundef_src_dec EF_src_dec V_src_dec defs1_src defs2_src = Some defs_src)
       (H1: globdef_list_sim defs1_src defs1_tgt)
       (H2: globdef_list_sim defs2_src defs2_tgt):
   exists defs_tgt,
-    link_globdef_list V_dec defs1_tgt defs2_tgt = Some defs_tgt /\
+    link_globdef_list fundef_tgt_dec EF_tgt_dec V_tgt_dec defs1_tgt defs2_tgt = Some defs_tgt /\
     globdef_list_sim defs_src defs_tgt.
 Proof.
   apply globdef_list_sim_globdefs_sim in H1.
   apply globdef_list_sim_globdefs_sim in H2.
   unfold link_globdef_list in Hdefs_src.
   match goal with
-    | [H: context[link_globdefs ?V_dec ?defs1 ?defs2] |- _] =>
-      destruct (link_globdefs V_dec defs1 defs2) as [defs|] eqn:Hdefs; inv H
+    | [H: context[link_globdefs ?fundef_dec ?EF_dec ?V_dec ?defs1 ?defs2] |- _] =>
+      destruct (link_globdefs fundef_dec EF_dec V_dec defs1 defs2) as [defs|] eqn:Hdefs; inv H
   end.
   exploit link_globdefs_sim; eauto. intros [defs_tgt [Hdefs_tgt Hsim]].
   unfold link_globdef_list. rewrite Hdefs_tgt. eexists. split; eauto.
@@ -238,13 +278,13 @@ Proof.
 Qed.
 
 Lemma link_program_sim
-      (p1_src p2_src:program (AST.fundef F_src) V)
-      (p1_tgt p2_tgt:program (AST.fundef F_tgt) V)
-      p_src (Hm_src: link_program V_dec p1_src p2_src = Some p_src)
+      (p1_src p2_src:program Fundef_src V_src)
+      (p1_tgt p2_tgt:program Fundef_tgt V_tgt)
+      p_src (Hm_src: link_program fundef_src_dec EF_src_dec V_src_dec p1_src p2_src = Some p_src)
       (H1: program_sim p1_src p1_tgt)
       (H2: program_sim p2_src p2_tgt):
   exists m_tgt,
-    link_program V_dec p1_tgt p2_tgt = Some m_tgt /\
+    link_program fundef_tgt_dec EF_tgt_dec V_tgt_dec p1_tgt p2_tgt = Some m_tgt /\
     program_sim p_src m_tgt.
 Proof.
   destruct p1_src as [defs1_src main1_src].
@@ -255,7 +295,7 @@ Proof.
   unfold link_program in *. simpl in *. subst.
   destruct ((main1_tgt =? main2_tgt)%positive) eqn:Hmain; [|inv Hm_src].
   apply Pos.eqb_eq in Hmain. subst.
-  destruct (link_globdef_list V_dec defs1_src defs2_src) as [defs_src|] eqn:Hdef_src; inv Hm_src.
+  destruct (link_globdef_list fundef_src_dec EF_src_dec V_src_dec defs1_src defs2_src) as [defs_src|] eqn:Hdef_src; inv Hm_src.
   exploit link_globdef_list_sim; eauto.
   intros [defs_tgt [Hdefs_tgt Hsim]].
   rewrite Hdefs_tgt. eexists. split; eauto.
@@ -265,12 +305,12 @@ Qed.
 
 Section INITIALIZE.
 
-Variable (p_src: program (AST.fundef F_src) V).
-Variable (p_tgt: program (AST.fundef F_tgt) V).
+Variable (p_src: program Fundef_src V_src).
+Variable (p_tgt: program Fundef_tgt V_tgt).
 Variable (Hp: program_sim p_src p_tgt).
 
 Lemma program_sim_match_program:
-  match_program globfun_sim eq nil p_src.(prog_main) p_src p_tgt.
+  match_program globfun_sim V_sim nil p_src.(prog_main) p_src p_tgt.
 Proof.
   destruct Hp as [Hdefs Hmain].
   unfold match_program. split; eauto.
@@ -280,11 +320,13 @@ Proof.
   destruct v1 as [var1 g1], v2 as [var2 g2]. simpl in *. subst.
   inv H2.
   - constructor. auto.
-  - destruct v. constructor. auto.
+  - destruct v_src. unfold transf_globvar in Hv. simpl in Hv.
+    destruct (transf_V gvar_info) eqn:Hinfo; inv Hv. simpl in *.
+    constructor. auto.
 Qed.
 
 Lemma globalenvs_match:
-  Genv.match_genvs globfun_sim eq nil (Genv.globalenv p_src) (Genv.globalenv p_tgt).
+  Genv.match_genvs globfun_sim V_sim nil (Genv.globalenv p_src) (Genv.globalenv p_tgt).
 Proof.
   generalize program_sim_match_program. intro Hmatch.
   eapply Genv.globalenvs_match; eauto; auto.
@@ -308,9 +350,9 @@ Proof.
 Qed.
 
 Theorem find_funct_ptr_match:
-  forall (b : block) (f : AST.fundef F_src),
+  forall (b : block) (f : Fundef_src),
   Genv.find_funct_ptr (Genv.globalenv p_src) b = Some f ->
-  exists tf : AST.fundef F_tgt,
+  exists tf : Fundef_tgt,
   Genv.find_funct_ptr (Genv.globalenv p_tgt) b = Some tf /\ globfun_sim f tf.
 Proof.
   generalize program_sim_match_program. intros Hmatch b f Hf.
